.

pure/Data.v
@@ -6,82 +6,9 @@ Require Import Coq.micromega.Lia.
 Require Import DschingisKhan.pure.MyStructures.
 Require Import DschingisKhan.pure.MyUtilities.
 
-Module BinTree.
+Module BinaryTrees.
 
   Import ListNotations EqFacts MyUtilities BasicSetoidTheory BasicPosetTheory.
-
-  Section INDICES_OF_BINARY_TREES.
-
-  Inductive dir_t : Set :=
-  | Dir_left : dir_t
-  | Dir_right : dir_t
-  .
-
-  Definition index_t : Set :=
-    list dir_t
-  .
-
-  Definition encoding_index (idx : index_t) : nat :=
-    fold_right (dir_t_rect (fun _ => nat -> nat) (fun acc : nat => 2 * acc) (fun acc : nat => 2 * acc + 1)) 1 idx
-  .
-
-  Lemma encoding_index_unfold (idx : index_t) :
-    encoding_index idx =
-    match idx with
-    | [] => 1
-    | Dir_left :: idx' => 2 * encoding_index idx'
-    | Dir_right :: idx' => 2 * encoding_index idx' + 1
-    end.
-  Proof with eauto.
-    induction idx as [ | [ | ] idx IH]; simpl...
-  Qed.
-
-  Lemma decoding_index :
-    forall code : nat,
-    {idx : index_t | code <> 0 -> encoding_index idx = code}.
-  Proof with lia || eauto.
-    strong_rec. intros [ | n']; [exists ([]); contradiction | set (n := S n')].
-    destruct n' as [ | n'']; intros acc_hyp.
-    - exists ([])...
-    - assert (claim1 := Nat.div_mod n 2 (S_eq_0_elim 1)).
-      destruct (Nat.mod_bound_pos n 2 (le_intro_0_le_n n) (le_S 1 1 (le_n 1))) as [claim2 claim3].
-      assert (claim4 : leq (n / 2) n).
-      { apply le_implies_leq... }
-      assert (claim5 : n / 2 <> n)...
-      assert (claim6 : n / 2 <> 0)...
-      destruct (acc_hyp (n / 2) claim4 claim5) as [idx H_idx].
-      destruct (n mod 2) as [ | [ | n_mod_2]] eqn: H_obs...
-      { exists (Dir_left :: idx); rewrite encoding_index_unfold... }
-      { exists (Dir_right :: idx); rewrite encoding_index_unfold... }
-  Qed.
-
-  Lemma encoding_index_range :
-    forall code : nat,
-    (exists idx : index_t, encoding_index idx = code) <-> code <> 0.
-  Proof with lia || eauto.
-    intros n; split.
-    - intros [idx H_idx]; subst n; induction idx as [ | [ | ] idx IH]; simpl...
-    - intros H_n_ne_0. destruct (decoding_index n) as [idx H_idx]...
-  Qed.
-
-  Lemma encoding_index_injective :
-    forall idx1 : index_t,
-    forall idx2 : index_t,
-    encoding_index idx1 = encoding_index idx2 ->
-    idx1 = idx2.
-  Proof with lia || eauto.
-    assert (claim1 : forall idx : index_t, encoding_index idx > 0).
-    { intros idx. enough (to_show : encoding_index idx <> 0)... pose (proj1 (encoding_index_range (encoding_index idx)))... }
-    induction idx1 as [ | d1 idx1 IH]; destruct idx2 as [ | d2 idx2]...
-    - pose (claim1 idx2); rewrite encoding_index_unfold; destruct d2; simpl...
-    - pose (claim1 idx1); rewrite encoding_index_unfold; destruct d1; simpl...
-    - rewrite encoding_index_unfold with (idx := d1 :: idx1).
-      rewrite encoding_index_unfold with (idx := d2 :: idx2).
-      destruct d1; destruct d2...
-      all: intros H_eq; apply eq_congruence, IH...
-  Qed.
-
-  End INDICES_OF_BINARY_TREES.
 
   Inductive bintree (Elem : Type) : Type :=
   | BT_null : bintree Elem
@@ -91,106 +18,79 @@ Module BinTree.
   Global Arguments BT_null {Elem}.
   Global Arguments BT_node {Elem}.
 
-  Definition btctx (Elem : Type) : Type :=
-    list (dir_t * (Elem * bintree Elem))
+  Section INDICES_OF_BINARY_TREES.
+
+  Inductive dir_t : Set :=
+  | Dir_left : dir_t
+  | Dir_right : dir_t
   .
 
-  Inductive btctx_spec {Elem : Type} (sub_t : bintree Elem) : btctx Elem -> bintree Elem -> Prop :=
-  | CtxSpec_top
-    : btctx_spec sub_t [] sub_t
-  | CtxSpec_left c_l t_l e t_r
-    (H_l : btctx_spec sub_t c_l t_l)
-    : btctx_spec sub_t (c_l ++ [(Dir_left, (e, t_r))]) (BT_node t_l e t_r)
-  | CtxSpec_right c_r t_l e t_r
-    (H_r : btctx_spec sub_t c_r t_r)
-    : btctx_spec sub_t (c_r ++ [(Dir_right, (e, t_l))]) (BT_node t_l e t_r)
+  Definition encode (ds : list dir_t) : nat :=
+    fold_left (fun code : nat => dir_t_rect (fun _ => nat) (2 * code + 1) (2 * code + 2)) ds 0
   .
 
-  Local Hint Constructors btctx_spec : core.
+  Lemma decode (code : nat) :
+    {ds : list dir_t | encode ds = code}.
+  Proof with lia || eauto.
+    induction code as [[ | n'] IH] using Wf_nat.lt_wf_rect1.
+    - exists ([])...
+    - set (code := S n').
+      destruct (code mod 2) as [ | [ | code_mod_2]] eqn: H_obs.
+      + assert (claim1 : code = 2 * ((code - 2) / 2) + 2).
+        { apply (positive_even code ((code - 2) / 2))... }
+        assert (claim2 : (code - 2) / 2 < code)...
+        destruct (IH ((code - 2) / 2) claim2) as [ds H_ds].
+        exists (ds ++ [Dir_right]).
+        unfold encode. rewrite fold_left_last. unfold dir_t_rect at 1.
+        unfold encode in H_ds. rewrite H_ds...
+      + assert (claim1 : code = 2 * ((code - 1) / 2) + 1).
+        { apply (positive_odd code ((code - 1) / 2))... }
+        assert (claim2 : (code - 1) / 2 < code)...
+        destruct (IH ((code - 1) / 2) claim2) as [ds H_ds].
+        exists (ds ++ [Dir_left]).
+        unfold encode. rewrite fold_left_last. unfold dir_t_rect at 1.
+        unfold encode in H_ds. rewrite H_ds...
+      + pose (Nat.mod_bound_pos code 2)...
+  Defined.
 
-  Lemma btctx_spec_refl {Elem : Type} (root : bintree Elem) :
-    btctx_spec root [] root.
-  Proof.
-    constructor 1.
+(*
+  Compute (proj1_sig (decode 14)).
+  (* = [Dir_right; Dir_right; Dir_right] *)
+  Compute (proj1_sig (decode 15)).
+  (* = [Dir_left; Dir_left; Dir_left; Dir_left] *)
+  Compute (proj1_sig (decode 16)).
+  (* = [Dir_left; Dir_left; Dir_left; Dir_right] *)
+*)
+
+  Lemma encodex_inj :
+    forall ds1 : list dir_t,
+    forall ds2 : list dir_t,
+    encode ds1 = encode ds2 ->
+    ds1 = ds2.
+  Proof with lia || eauto.
+    unfold encode; intros ds1 ds2. do 2 rewrite <- fold_left_rev_right.
+    intros H_eq; apply list_rev_inj; revert H_eq.
+    generalize (rev ds2) as xs2. generalize (rev ds1) as xs1. clear ds1 ds2.
+    set (myF := fold_right (fun (y : dir_t) (x : nat) => dir_t_rect (fun _ : dir_t => nat) (2 * x + 1) (2 * x + 2) y) 0).
+    induction xs1 as [ | x1 xs1 IH]; destruct xs2 as [ | x2 xs2]; simpl...
+    - destruct x2; simpl dir_t_rect...
+    - destruct x1; simpl dir_t_rect...
+    - destruct x1; destruct x2; simpl dir_t_rect...
+      all: intros H_eq; assert (claim1 : myF xs1 = myF xs2)...
+      all: apply f_equal...
   Qed.
 
-  Lemma btctx_spec_trans {Elem : Type} (root : bintree Elem) :
-    forall t1 : bintree Elem,
-    forall c1 : btctx Elem,
-    btctx_spec t1 c1 root ->
-    forall t2 : bintree Elem,
-    forall c2 : btctx Elem,
-    btctx_spec t2 c2 t1 ->
-    btctx_spec t2 (c2 ++ c1) root.
-  Proof.
-    intros t1 c1 X1; induction X1; intros t2 c2 X2; simpl.
-    - rewrite app_nil_r; exact X2.
-    - rewrite app_assoc; constructor 2; apply IHX1; exact X2.
-    - rewrite app_assoc; constructor 3; apply IHX1; exact X2.
-  Qed.
+  End INDICES_OF_BINARY_TREES.
 
-  Definition recover_step_aux {Elem : Type} (d : dir_t) (e : Elem) (t : bintree Elem) : bintree Elem -> bintree Elem :=
-    match d with
-    | Dir_left => fun t_l : bintree Elem => BT_node t_l e t 
-    | Dir_right => fun t_r : bintree Elem => BT_node t e t_r
+  Fixpoint option_subtree {A : Type} (ds : list dir_t) (t : bintree A) : option (bintree A) :=
+    match ds with
+    | [] => Some t
+    | d :: ds' =>
+      match t with
+      | BT_null => None
+      | BT_node l e r => option_subtree ds' (dir_t_rect (fun _ => bintree A) l r d)
+      end
     end
   .
 
-  Definition recover_step {Elem : Type} : (dir_t * (Elem * bintree Elem)) -> bintree Elem -> bintree Elem :=
-    fun it : dir_t * (Elem * bintree Elem) =>
-    uncurry (recover_step_aux (fst it)) (snd it)
-  .
-
-  Definition recover {Elem : Type} (sub_t : bintree Elem) (c : btctx Elem) : bintree Elem :=
-    fold_right recover_step sub_t (rev c)
-  .
-
-  Lemma recover_unfold {Elem : Type} (sub_t : bintree Elem) c :
-    recover sub_t c =
-    match c with
-    | [] => sub_t
-    | (Dir_left, (e, t_r)) :: c_l => recover (BT_node sub_t e t_r) c_l
-    | (Dir_right, (e, t_l)) :: c_r => recover (BT_node t_l e sub_t) c_r
-    end.
-  Proof with eauto.
-    unfold recover at 1; rewrite fold_left_rev_right with (f := recover_step).
-    destruct c as [ | [[ | ] [e t]] c]; simpl...
-    all: unfold recover at 1; rewrite fold_left_rev_right with (f := recover_step)...
-  Qed.
-
-  Lemma recover_last {Elem : Type} (sub_t : bintree Elem) c d e t :
-    recover sub_t (c ++ [(d, (e, t))]) =
-    match d with
-    | Dir_left => BT_node (recover sub_t c) e t 
-    | Dir_right => BT_node t e (recover sub_t c)
-    end.
-  Proof.
-    unfold recover at 1; rewrite list_rev_cons, fold_right_unfold; now destruct d.
-  Qed.
-
-  Theorem btctx_spec_recover {Elem : Type} sub_t c (root : bintree Elem) :
-    btctx_spec sub_t c root <-> recover sub_t c = root.
-  Proof with eauto.
-    split.
-    - intros X; induction X; simpl...
-      all: rewrite recover_last, IHX...
-    - intros H_eq; subst root; revert sub_t.
-      pattern c; revert c; apply list_reversed_induction...
-      intros idx [[ | ] [e t]] IH sub_t; rewrite recover_last...
-  Qed.
-
-  Lemma btctx_spec_left {Elem : Type} c t_l e t_r (root : bintree Elem) :
-    btctx_spec (BT_node t_l e t_r) c root <-> btctx_spec t_l ((Dir_left, (e, t_r)) :: c) root.
-  Proof.
-    do 2 rewrite btctx_spec_recover.
-    now rewrite recover_unfold with (c := (Dir_left, (e, t_r)) :: c).
-  Qed.
-
-  Lemma btctx_spec_right {Elem : Type} c t_l e t_r (root : bintree Elem) :
-    btctx_spec (BT_node t_l e t_r) c root <-> btctx_spec t_r ((Dir_right, (e, t_l)) :: c) root.
-  Proof.
-    do 2 rewrite btctx_spec_recover.
-    now rewrite recover_unfold with (c := (Dir_right, (e, t_l)) :: c).
-  Qed.
-
-End BinTree.
+End BinaryTrees.
